more strong progress

theories/sessiontypes/progress.v
@@ -247,330 +247,32 @@ Proof.
     by apply NNPP.
 Qed.
 
-Lemma active_progress es h x :
-  invariant es h -> active x es h -> ∃ (es' : list expr) (h' : heap), step es h es' h'.
+Definition obj_refs (es : list expr) (h : heap) (x : object) : gset object. Admitted.
+
+Lemma obj_refs_state_inv' es h x Δ :
+  state_inv es h x Δ ⊢ ∃ Σ, ⌜⌜ obj_refs es h x = dom (gset object) Σ ⌝⌝ ∗ own Σ.
 Proof.
-  intros (g & Hwf & Hvs). revert x.
-  eapply (cgraph_ind' (waiting es h) g (λ x,
-    active x es h → ∃ (es' : list expr) (h' : heap), step es h es' h'));
-    [solve_proper|eauto|].
-  intros x Hind_out Hind_in Hactive.
-  (* Get the invariant for x *)
-  pose proof (Hvs x) as Hx.
-  (* Case analyze whether x is a channel or a thread *)
-  destruct x as [i|i]; simpl in *.
-  - (* Thread *)
-    destruct Hactive as (e & He & Heneq). (* Thread is active, so must have expression in thread pool *)
-    rewrite He in Hx. (* We can conclude that this expression is well-typed wrt out edges *)
-    apply pure_sep_holds in Hx as [Hinl Hx].
-    eapply prim_simple_adequacy in Hx as Hx'; last eapply rtyped_inner.
-    (* Case analyze whether it's a value or pure step or channel op  *)
-    destruct Hx' as [(v & ->)|Hx'].
-    {
-      (* Value *)
-      eapply prim_simple_adequacy; first done.
-      simpl. rewrite val_typed_val_typed'. simpl.
-      iIntros (->). simplify_eq.
-    }
-    (* Expr in context *)
-    destruct Hx' as (k' & e0 & Hctx & -> & Hcases).
-    rewrite ->rtyped0_ctx in Hx; eauto.
-    apply exists_holds in Hx as [t Hx].
-    apply sep_holds in Hx as (Σ1&Σ2&Hout&Hdisj&Het&Hctxt).
-    destruct Hcases as [H|[H|[H|[H|H]]]].
-    * (* Pure step *)
-      destruct H as [e' H].
-      eexists _,_.
-      econstructor. econstructor; last done.
-      econstructor; eauto.
-      econstructor. done.
-    * (* Recv *)
-      destruct H as [v ->].
-      revert Het.
-      Ltac model := repeat
-        (setoid_rewrite pure_sep_holds || setoid_rewrite exists_holds
-        || setoid_rewrite own_holds || setoid_rewrite val_typed_val_typed'
-        || setoid_rewrite sep_holds).
-      model.
-      intros (t' & r & -> & [c b] & -> & Het). simpl in *.
-      assert (out_edges g (Thread i) !! Chan c ≡ Some (b, RecvT t' r)) as HH.
-      {
-        rewrite Hout -Het. erewrite lookup_union_Some_l; first done.
-        rewrite lookup_singleton. done.
-      }
+Admitted.
 
-      pose proof (out_edges_in_labels _ _ _ _ HH) as [x Hin].
-
-      assert (∃ buf, h !! (c,b) = Some buf) as [buf Hbuf].
-      {
-        pose proof (Hvs (Chan c)) as Hc.
-        eapply prim_simple_adequacy; first done.
-        iIntros "H". simpl.
-        iDestruct "H" as (σs Hinlc) "H".
-        iDestruct (bufs_typed_wlog true b with "H") as "H".
-        assert (σs !! b ≡ Some (RecvT t' r)) as ->.
-        { eapply map_to_multiset_lookup. rewrite <-Hinlc, Hin. done. }
-        unfold bufs_typed.
-        iDestruct "H" as (rest) "[H1 H2]".
-        destruct (h !! (c,b)) eqn:E; eauto.
-      }
-
-      destruct buf.
-      {
-        eapply Hind_out; eauto.
-        - unfold waiting, thread_waiting; eauto 10.
-        - simpl. exists b. rewrite Hbuf //.
-      }
-
-      eexists _,_.
-      econstructor; econstructor; last done.
-      econstructor; first done.
-      eapply Recv_step. done.
-    * (* Send *)
-      destruct H as (v1 & v2 & ->).
-      revert Het. model.
-      intros (r & t' & -> & Σ3 & Σ4 & Σeq & Hdisj' & ([c b] & -> & Het1) & Het2).
-
-      assert (out_edges g (Thread i) !! Chan c ≡ Some (b, SendT t' r)) as HH.
-      {
-        rewrite <-Het1 in Σeq. rewrite ->Σeq in Hout. rewrite ->Σeq in Hdisj. clear Σeq.
-        rewrite Hout. erewrite lookup_union_Some_l; first done.
-        erewrite lookup_union_Some_l; first done.
-        rewrite lookup_singleton. done.
-      }
-
-      pose proof (out_edges_in_labels _ _ _ _ HH) as [x Hin].
-
-      assert (∃ buf, h !! (c,negb b) = Some buf) as [buf Hbuf].
-      {
-        pose proof (Hvs (Chan c)) as Hc.
-        eapply prim_simple_adequacy; first done.
-        simpl.
-        iIntros "H". iDestruct "H" as (σs Hinlc) "H".
-        iDestruct (bufs_typed_wlog true b with "H") as "H".
-        assert (σs !! b ≡ Some (SendT t' r)) as ->.
-        { eapply map_to_multiset_lookup. rewrite <-Hinlc, Hin. done. }
-        unfold bufs_typed.
-        iDestruct "H" as (rest) "[H1 H2]".
-        destruct (h !! (c,b)) eqn:E; eauto. simpl.
-        destruct (h !! (c,negb b)) eqn:F; eauto. simpl.
-        destruct (σs !! negb b) eqn:G; eauto.
-        iDestruct "H2" as "%". apply dual_end_inv in H. subst.
-        destruct l; eauto. simpl.
-        iDestruct "H1" as "%". inversion H.
-      }
-
-      eexists _,_.
-      econstructor; econstructor; last done.
-      econstructor; first done.
-      eapply Send_step. done.
-    * (* Fork *)
-      destruct H as (v & ->).
-      destruct (heap_fresh h) as [ii HH].
-      eexists _,_.
-      econstructor; econstructor; last done.
-      econstructor; eauto.
-      eapply Fork_step; eauto.
-    * (* Close *)
-      destruct H as (v & ->).
-      revert Het. model.
-      intros (-> & ([c b] & -> & Het)).
-      assert (out_edges g (Thread i) !! (Chan c) ≡ Some (b,EndT)) as HH.
-      {
-        rewrite Hout -Het. erewrite lookup_union_Some_l; eauto.
-        rewrite lookup_singleton. done.
-      }
-
-      pose proof (out_edges_in_labels _ _ _ _ HH) as [x Hx].
-
-      assert (h !! (c,b) = Some []).
-      {
-        pose proof (Hvs (Chan c)) as Hc.
-        eapply prim_simple_adequacy; first done. simpl.
-        iIntros "H". iDestruct "H" as (σs Hinlc) "H".
-        iDestruct (bufs_typed_wlog true b with "H") as "H".
-        assert (σs !! b ≡ Some EndT) as ->.
-        { eapply map_to_multiset_lookup. rewrite <-Hinlc, Hx. done. }
-        unfold bufs_typed.
-        iDestruct "H" as (rest) "[H1 H2]".
-        destruct (h !! (c,b)) eqn:E; eauto.
-        simpl. destruct l; simpl; eauto.
-      }
-
-      eexists _,_.
-      econstructor; econstructor; last done.
-      econstructor; first done.
-      eapply Close_step. done.
-  - (* Channel *)
-    destruct Hactive as (b & Hib).
-    apply exists_holds in Hx as [σs Hx].
-    apply pure_sep_holds in Hx as [Hinl Hx].
-    eapply holds_entails in Hx; last by eapply (bufs_typed_wlog true b).
-    destruct Hib as [buf Hbuf].
-    rewrite Hbuf in Hx.
-    destruct (σs !! b) as [σ1|] eqn:E; last first.
-    { eapply prim_simple_adequacy; first done.
-      rewrite /bufs_typed /=. iIntros "H".
-      by iDestruct "H" as (?) "[% ?]". }
-    erewrite map_to_multiset_Some in Hinl; eauto.
-
-    destruct (classic (∃ c q, out_edges g (Chan c) !! Chan i ≡ Some q)) as [(c & q & Hc)|Hnc].
-    { (* This thing will handle the case of a chan-chan reference for us *)
-      eapply (Hind_in (Chan c)); simpl; eauto. { rewrite /waiting. naive_solver. }
-      destruct (h !! (c,true)) eqn:Q; eauto.
-      destruct (h !! (c,false)) eqn:Q'; eauto.
-      assert (out_edges g (Chan c) = ∅) as H.
-      {
-        eapply prim_empty_adequacy; first exact (Hvs (Chan c)).
-        iIntros "H". simpl. rewrite Q Q' /bufs_typed /=.
-        iDestruct "H" as (σs' ? ?) "[H1 H2]".
-        destruct (σs' !! true),(σs' !! false); eauto.
-      }
-      rewrite H lookup_empty in Hc. inversion Hc.
-    }
-    (* Since the chan has a buffer, there exists somebody holding a ref to this chan *)
-    (* If the other one is a chan, we're done *)
-    assert (∃ y, out_edges g y !! (Chan i) ≡ Some (b,σ1)) as [[] Hy];
-      first (eapply in_labels_out_edges; eauto); last (exfalso; eauto).
-    (* The one holding the ref to the chan is a thread *)
-    pose proof (Hvs (Thread n)) as Hn. simpl in Hn.
-    eapply pure_sep_holds in Hn as [? Hn].
-    destruct (es !! n) eqn:En; last first.
-    {
-      eapply emp_holds in Hn.
-      eapply map_empty_equiv_eq in Hn.
-      rewrite Hn in Hy. rewrite lookup_empty in Hy. inversion Hy.
-    }
-    destruct (classic (waiting es h (Thread n) (Chan i) (b, σ1))) as [w|n0]; last first.
-    {
-      (* The thread is not blocked on the chan (but could be blocked on another chan) *)
-      eapply Hind_in; eauto. (* We need to show that the thread hasn't terminated with a unit value *)
-      simpl. exists e. split; eauto. intros ->.
-      simpl in Hn.
-      eapply affinely_pure_holds in Hn as [].
-      eapply map_empty_equiv_eq in H0.
-      rewrite H0 lookup_empty in Hy. inversion Hy.
-    }
-    (* The thread is blocked on the chan *)
-    unfold waiting in w.
-    destruct w as (i0 & j & ? & ? & Htw). simplify_eq.
-    unfold thread_waiting in Htw.
-    destruct Htw as (b' & k & Hk & Hi0 & Hjb).
-    rewrite Hi0 in En. simplify_eq.
-    rewrite ->rtyped0_ctx in Hn; eauto.
-    eapply exists_holds in Hn as [t Hn].
-    eapply sep_holds in Hn as (?&?&?&?&?&?).
-    simpl in H2.
-    eapply exists_holds in H2 as [t' H2].
-    eapply exists_holds in H2 as [r H2].
-    eapply pure_sep_holds in H2 as [-> H2].
-    eapply exists_holds in H2 as [r0 H2].
-    eapply pure_sep_holds in H2 as [? H2]. simplify_eq.
-    eapply own_holds in H2.
-    assert (Some (b',RecvT t' r) ≡ Some (b,σ1)).
-    {
-      rewrite <- Hy.
-      rewrite H0.
-      rewrite <- H2.
-      rewrite lookup_union lookup_singleton.
-      destruct (x0 !! Chan j) eqn:Q; simpl.
-      - rewrite Q. simpl. done.
-      - rewrite Q. simpl. done.
-    }
-    inversion H4. inversion H7. simpl in *.
-    apply leibniz_equiv in H8.
-    simplify_eq.
-    rewrite Hbuf in Hjb. simplify_eq.
-    simpl in Hx.
-    eapply exists_holds in Hx as [rest Hx].
-    eapply pure_sep_holds in Hx as [-> Hx].
-    simpl in Hx.
-    destruct (h !! (j,negb b)) eqn:Q; last first.
-    {
-      simpl in Hx. destruct (σs !! negb b).
-      - eapply false_holds in Hx as [].
-      - eapply affinely_pure_holds in Hx as [].
-        rewrite <-H9 in H6.
-        rewrite ->dual_recv in H6. inversion H6.
-    }
-    simpl in Hx.
-    destruct (σs !! negb b) eqn:Q2; last first.
-    { eapply false_holds in Hx as []. }
-    assert (delete b σs !! negb b = Some c) as HHH.
-    { rewrite lookup_delete_ne //. by destruct b. }
-    erewrite map_to_multiset_Some in Hinl; eauto.
-
-    rewrite ->(comm (⋅)), <-assoc in Hinl; last apply _.
-
-    assert (∃ z, out_edges g z !! (Chan j) ≡ Some (negb b, c)) as [z Hzout].
-    {
-      eapply in_labels_out_edges; eauto.
-    }
-    clear HHH.
-    destruct z; last (exfalso; eauto).
-    pose proof (Hvs (Thread n)) as Hz. simpl in Hz.
-    eapply pure_sep_holds in Hz as [? Hz].
-    destruct (es !! n) eqn:R; last first.
-    {
-      eapply emp_holds in Hz.
-      eapply map_empty_equiv_eq in Hz.
-      rewrite Hz in Hzout. rewrite lookup_empty in Hzout.
-      inversion Hzout.
-    }
-    destruct (classic (waiting es h (Thread n) (Chan j) (negb b, c))) as [w|n0]; last first.
-    {
-      eapply Hind_in; eauto.
-      simpl. exists e. split; eauto.
-      intros ->.
-      simpl in Hz.
-      eapply affinely_pure_holds in Hz as [].
-      eapply map_empty_equiv_eq in H6.
-      rewrite H6 in Hzout.
-      rewrite lookup_empty in Hzout.
-      inversion Hzout.
-    }
-    unfold waiting in w.
-    destruct w as (? & ? & ? & ? & Htw). simplify_eq.
-    unfold thread_waiting in Htw.
-    destruct Htw as (b' & ? & ? & HH & Hjb).
-    rewrite HH in R. simplify_eq.
-    rewrite ->rtyped0_ctx in Hz; eauto.
-    eapply exists_holds in Hz as [t Hz].
-    eapply sep_holds in Hz as (?&?&?&?&QQ&?).
-    simpl in *.
-    eapply exists_holds in QQ as [? QQ].
-    eapply exists_holds in QQ as [? QQ].
-    eapply pure_sep_holds in QQ as [-> QQ].
-    eapply exists_holds in QQ as [? QQ].
-    eapply pure_sep_holds in QQ as [? QQ]. simplify_eq.
-    eapply own_holds in QQ.
-    assert (Some (b',RecvT x6 x7) ≡ Some (negb b,c)).
-    {
-      rewrite <- Hzout.
-      rewrite H8.
-      rewrite <- QQ.
-      rewrite lookup_union lookup_singleton.
-      destruct (x5 !! Chan x2) eqn:Q'; simpl.
-      - rewrite Q'. simpl. done.
-      - rewrite Q'. simpl. done.
-    }
-    inversion H12. simplify_eq.
-    inversion H15. simpl in *. apply leibniz_equiv in H13.
-    simplify_eq.
-    rewrite Hjb in Q. simplify_eq.
-    simpl in Hx.
-    eapply affinely_pure_holds in Hx as [].
-    inversion H7. simpl in *.
-    inversion H18; simplify_eq. inversion H14.
-    simplify_eq. rewrite ->dual_recv in H16. inversion H16.
+Lemma obj_refs_state_inv es h x Δ Σ :
+  holds (state_inv es h x Δ) Σ -> obj_refs es h x = dom (gset object) Σ.
+Proof.
+  intros HH. eapply holds_entails in HH; last apply obj_refs_state_inv'.
+  eapply exists_holds in HH as [Σ' HH].
+  eapply pure_sep_holds in HH as [HH1 HH2].
+  eapply own_holds in HH2. rewrite HH1 HH2 //.
 Qed.
-
-Definition chan_refs (es : list expr) (h : heap) (x : object) : gset chan. Admitted.
 
 Inductive reachable (es : list expr) (h : heap) : object → Prop :=
   | Thread_step_reachable i : can_stepi i es h → reachable es h (Thread i)
   | Thread_waiting_reachable i c : reachable es h (Chan c) → thread_waiting es h i c → reachable es h (Thread i)
-  | Chan_ref_reachable c x : c ∈ chan_refs es h x → reachable es h x → reachable es h (Chan c).
+  | Chan_ref_reachable c x : (Chan c) ∈ obj_refs es h x → reachable es h x → reachable es h (Chan c).
+
+Lemma dom_lookup_Some_equiv `{Countable A} `{Equiv B} (m : gmap A B) (x : A) (y : B) :
+  m !! x ≡ Some y -> x ∈ dom (gset A) m.
+Proof.
+  intros HH. inversion HH. subst. eapply elem_of_dom. rewrite -H1 //.
+Qed.
 
 Lemma strong_progress es h x :
   invariant es h -> active x es h -> reachable es h x.
@@ -728,8 +430,9 @@ Proof.
 
     destruct (classic (∃ c q, out_edges g (Chan c) !! Chan i ≡ Some q)) as [(c & q & Hc)|Hnc].
     { (* This thing will handle the case of a chan-chan reference for us *)
-      eapply Chan_ref_reachable.
-      { admit. }
+      eapply (Chan_ref_reachable _ _ _ (Chan c)).
+      { erewrite obj_refs_state_inv; eauto.
+        eapply dom_lookup_Some_equiv; eauto. }
       eapply (Hind_in (Chan c)); simpl; eauto. { rewrite /waiting. naive_solver. }
       destruct (h !! (c,true)) eqn:Q; eauto.
       destruct (h !! (c,false)) eqn:Q'; eauto.
@@ -756,10 +459,10 @@ Proof.
       rewrite Hn in Hy. rewrite lookup_empty in Hy. inversion Hy.
     }
     destruct (classic (waiting es h (Thread n) (Chan i) (b, σ1))) as [w|n0]; last first.
-    {
-      (* The thread is not blocked on the chan (but could be blocked on another chan) *)
-      eapply Chan_ref_reachable.
-      { admit. }
+    { (* The thread is not blocked on the chan (but could be blocked on another chan) *)
+      eapply (Chan_ref_reachable _ _ _ (Thread n)).
+      { erewrite obj_refs_state_inv; eauto.
+        eapply dom_lookup_Some_equiv; eauto. }
       eapply Hind_in; eauto. (* We need to show that the thread hasn't terminated with a unit value *)
       simpl. exists e. split; eauto. intros ->.
       simpl in Hn.
@@ -835,6 +538,9 @@ Proof.
     }
     destruct (classic (waiting es h (Thread n) (Chan j) (negb b, c))) as [w|n0]; last first.
     {
+      eapply (Chan_ref_reachable _ _ _ (Thread n)).
+      { erewrite obj_refs_state_inv; eauto.
+        eapply dom_lookup_Some_equiv; eauto. }
       eapply Hind_in; eauto.
       simpl. exists e. split; eauto.
       intros ->.
@@ -879,6 +585,15 @@ Proof.
     inversion H7. simpl in *.
     inversion H18; simplify_eq. inversion H14.
     simplify_eq. rewrite ->dual_recv in H16. inversion H16.
+Qed.
+
+Lemma active_progress es h x :
+  invariant es h -> active x es h -> ∃ (es' : list expr) (h' : heap), step es h es' h'.
+Proof.
+  intros H1 H2.
+  cut (reachable es h x); eauto using strong_progress.
+  clear. induction 1; eauto.
+  destruct H as (es'&h'&?). exists es', h'. econstructor; eauto.
 Qed.
 
 Lemma global_progress es h :
